1. Basic eformat lemmas have been lifted up to MathUAdjMatGraph. 2. A new set of files, SpaceUAdjMatGraph1/2/3, have been created, which Import-Export SpaceAdjMatGraph1/2/3 and concoct theory about eformat + spatial rep 3. Three eformat lemmas needed PrimGG to work, so they have been moved into MathPrimGraph. They can be reused three times over. 4. SpacePrimGraph3 is now much lighter Make mst is clean.

prim/MathPrimGraph.v
@@ -148,6 +148,68 @@ simpl in *. destruct H1. auto. destruct H1; subst u; subst v. lia.
 all: apply H.
 Qed.
 
+Lemma eformat_evalid_vvalid:
+forall (g: PrimGG) u v, evalid g (eformat (u,v)) -> vvalid g u /\ vvalid g v.
+Proof.
+intros. apply evalid_strong_evalid in H.
+destruct (Z.lt_trichotomy u v).
+rewrite eformat1 in H. destruct H.
+rewrite (edge_src_fst g), (edge_dst_snd g) in H1; auto. simpl; lia.
+destruct H0.
+subst u. rewrite eformat1 in H. destruct H.
+rewrite (edge_src_fst g), (edge_dst_snd g) in H0; auto. simpl; lia.
+rewrite eformat2 in H. simpl in H; destruct H.
+rewrite (edge_src_fst g), (edge_dst_snd g) in H1; auto. simpl in H1.
+split; apply H1. simpl; lia.
+Qed.
+
+Lemma eformat_adj': forall (g : PrimGG) u v, evalid g (eformat (u,v)) -> adj_edge g (eformat (u,v)) u v.
+Proof.
+intros. split. apply (evalid_strong_evalid g); auto.
+destruct (Z.le_ge_cases u v).
+rewrite eformat1 in *. left. rewrite (edge_src_fst g), (edge_dst_snd g); auto. auto. auto.
+rewrite eformat2 in *. right. rewrite (edge_src_fst g), (edge_dst_snd g); auto. auto. auto.
+Qed.
+
+Lemma eformat_adj: forall (g: PrimGG) u v, adjacent g u v <-> evalid g (eformat (u,v)).
+Proof.
+intros. split. intros.
++
+destruct H. destruct H. destruct H.
+destruct H0; destruct H0. assert (x = (u,v)). {
+  rewrite (edge_src_fst g) in H0.
+  rewrite (edge_dst_snd g) in H2. rewrite <- H0, <- H2. destruct x; simpl; auto.
+} subst x.
+rewrite eformat1; auto. simpl.
+rewrite <- H0. rewrite <- H2 at 2. apply (undirected_edge_rep g); auto.
+assert (x = (v,u)). {
+  rewrite (edge_src_fst g) in H0; rewrite (edge_dst_snd g) in H2.
+  rewrite <- H0, <- H2. destruct x; simpl; auto.
+} subst x.
+rewrite eformat2. simpl. auto. simpl. rewrite <- H0. rewrite <- H2 at 2.
+apply (undirected_edge_rep g); auto.
++intros. destruct (Z.lt_trichotomy u v).
+rewrite eformat1 in H. 2: simpl; lia.
+assert (evalid g (u,v)). auto.
+exists (u,v). split. apply evalid_strong_evalid; auto. left.
+rewrite (edge_src_fst g), (edge_dst_snd g); auto.
+(*equal, repeat*)
+destruct H0. rewrite eformat1 in H. 2: simpl; lia.
+assert (evalid g (u,v)). auto.
+exists (u,v). split. apply evalid_strong_evalid; auto. left.
+rewrite (edge_src_fst g), (edge_dst_snd g); auto.
+rewrite eformat2 in H. 2: simpl; lia. simpl in H.
+assert (evalid g (v,u)). auto.
+exists (v,u). split. apply evalid_strong_evalid; auto.
+rewrite (edge_src_fst g), (edge_dst_snd g); auto.
+Qed.
+
+Corollary eformat_adj_elabel: forall (g: PrimGG) u v, adjacent g u v <-> elabel g (eformat (u,v)) < inf.
+Proof.
+intros. rewrite eformat_adj. apply evalid_inf_iff.
+Qed.
+
+
 (****************Edgeless graph again*****************)
 
 Section EDGELESS_MUGRAPH.
@@ -1088,42 +1150,5 @@ intros. unfold sublist. rewrite skipn_0. rewrite firstn_same. auto.
 rewrite <- ZtoNat_Zlength. lia.
 Qed.
 
-
-(* Eformat Lemmas have been put back here.
-   Sorry about moving them in the first place; 
-   that was an error in judgement. 
- *)
-Definition eformat (e: E) := if fst e <=? snd e then e else (snd e, fst e).
-
-Lemma eformat1: forall (e: E), fst e <= snd e -> eformat e = e.
-Proof. unfold eformat; intros. rewrite Zle_is_le_bool in H; rewrite H. auto. Qed.
-
-Lemma eformat2': forall (e: E), snd e < fst e -> eformat e = (snd e, fst e).
-Proof. unfold eformat; intros. rewrite <- Z.leb_gt in H; rewrite H. auto. Qed.
-
-Lemma eformat2: forall (e: E), snd e <= fst e -> eformat e = (snd e, fst e).
-Proof.
-  intros. apply Z.le_lteq in H. destruct H. rewrite eformat2'; auto. rewrite eformat1, H. rewrite <- H at 2. destruct e; auto. lia.
-Qed.
-
-Lemma eformat_eq:
-  forall u v a b, eformat (u,v) = eformat (a,b) -> ((u=a /\ v=b) \/ (u=b /\ v=a)).
-Proof.
-  intros. destruct (Z.le_ge_cases u v); destruct (Z.le_ge_cases a b).
-  rewrite eformat1, eformat1 in H. apply pair_equal_spec in H. left; auto. simpl; auto. simpl; auto. simpl; auto.
-  rewrite eformat1, eformat2 in H. simpl in H. apply pair_equal_spec in H. right; auto. simpl; auto. simpl; auto.
-  rewrite eformat2, eformat1 in H. simpl in H. apply pair_equal_spec in H. right; split; apply H. simpl; auto. simpl; auto.
-  rewrite eformat2, eformat2 in H. simpl in H. apply pair_equal_spec in H. left; split; apply H. simpl; auto. simpl; auto.
-Qed.
-
-Lemma eformat_symm:
-  forall u v, eformat (u,v) = eformat (v,u).
-Proof.
-  intros. destruct (Z.lt_trichotomy u v).
-  rewrite eformat1. rewrite eformat2. simpl; auto. simpl; lia. simpl; lia.
-  destruct H.
-  rewrite eformat1. rewrite eformat2. simpl; auto. simpl; lia. simpl; lia.
-  rewrite eformat2'. rewrite eformat1. simpl; auto. simpl; lia. simpl; lia.
-Qed.
 
 End MathPrimGraph.
