graph/SpaceUAdjMatGraph1.v
@@ -1,0 +1,57 @@
+Require Import VST.floyd.proofauto.
+Require Import CertiGraph.graph.graph_model.
+Require Import CertiGraph.graph.MathUAdjMatGraph.
+Require Export CertiGraph.graph.SpaceAdjMatGraph1.
+Require Import CertiGraph.lib.List_ext.
+
+Local Open Scope logic.
+
+Section Spatial_UAdjMat_Model_2.
+  (* Model 1 is for a heap-allocated graph,
+     where the graph is malloc-ed
+     by first malloc-ing a "spine" column of some size, 
+     and then malloc-ing a "row" into each cell
+     of the spine.       
+   *)
+
+Context {size : Z}.
+Context {inf : Z}.
+  
+Definition graph_to_symm_mat g :=
+  @graph_to_mat size g eformat.
+
+Lemma graph_to_mat_eq:
+  forall (g: AdjMatLG) i j, 0 <= i < size -> 0 <= j < size ->
+    (Znth i (Znth j (graph_to_symm_mat g))) = elabel g (eformat (i,j)).
+Proof.
+  intros.
+  symmetry. rewrite eformat_symm.
+  apply elabel_Znth_graph_to_mat; lia.
+Qed.
+
+Lemma graph_to_mat_symmetric:
+  forall (g: AdjMatLG) i j,
+    0 <= i < size -> 0 <= j < size ->
+    (Znth i (Znth j (graph_to_symm_mat g))) =
+    (Znth j (Znth i (graph_to_symm_mat g))).
+Proof.
+  intros. repeat rewrite graph_to_mat_eq; trivial.
+  f_equal. apply eformat_symm.
+Qed.
+
+Lemma graph_to_mat_inf:
+  forall (g: @AdjMatGG size inf) u v,
+    0 <= u < v ->
+    v < size ->
+    ~ evalid g (u,v) ->
+    Znth v (Znth u (graph_to_symm_mat g)) =
+    inf.
+Proof.
+  intros. unfold graph_to_symm_mat.
+  rewrite <- elabel_Znth_graph_to_mat; try lia.
+  rewrite eformat1.
+  apply (MathAdjMatGraph.invalid_edge_weight); auto.
+  simpl; lia.
+Qed.
+
+End Spatial_UAdjMat_Model_2.
