Makefile
@@ -44,7 +44,7 @@ GRAPH_FILES = \
   graph_isomorphism.v undirected_graph.v undirected_uf_lemmas.v \
   MathAdjMatGraph.v SpaceAdjMatGraph1.v SpaceAdjMatGraph2.v SpaceAdjMatGraph3.v \
   path_cost.v \
-  MathUAdjMatGraph.v
+  MathUAdjMatGraph.v SpaceUAdjMatGraph1.v SpaceUAdjMatGraph2.v SpaceUAdjMatGraph3.v
 
   # 1 = noncontiguous
   # 2 = contiguous 1-d
